Launchbury/CoCallAnalysisImpl.thy
@@ -86,7 +86,7 @@ nominal_function
 where
   "cCCexp (GVar b x) = (\<Lambda> n . (AE_singleton x \<cdot> (up \<cdot> n), \<bottom>))"
 | "cCCexp (Lam [x]. e) = (\<Lambda> n . combined_restrict (fv (Lam [x]. e)) (fst (cCCexp e\<cdot>(pred\<cdot>n)), predCC (fv (Lam [x]. e)) (\<Lambda> a. snd(cCCexp e\<cdot>a))\<cdot>n))"
-| "cCCexp (App e x) = (\<Lambda> n . (fst (cCCexp e\<cdot>(inc\<cdot>n)) \<squnion> (AE_singleton x \<cdot> (up \<cdot> 0)), snd (cCCexp e\<cdot>(inc\<cdot>n)) \<squnion> ccProd (fv e) {x}))"
+| "cCCexp (App e x) = (\<Lambda> n . (fst (cCCexp e\<cdot>(inc\<cdot>n)) \<squnion> (AE_singleton x \<cdot> (up \<cdot> 0)), snd (cCCexp e\<cdot>(inc\<cdot>n)) \<squnion> ccProd {x} (insert x (fv e))))"
 | "cCCexp (Let \<Gamma> e) = (\<Lambda> n . combined_restrict (fv (Let \<Gamma> e)) (CoCallArityAnalysis.cccFix cCCexp \<Gamma> \<cdot> (cCCexp e \<cdot> n)))"
 proof-
 case goal1
@@ -158,7 +158,7 @@ unfolding Aexp_def CCexp_def Afix_def by (simp add: beta_cfun)+
 lemma CCexp_simps[simp]:
   "CCexp (GVar b x)\<cdot>n = \<bottom>"
   "CCexp (Lam [x]. e)\<cdot>n = predCC (fv (Lam [x]. e)) (CCexp e)\<cdot>n"
-  "CCexp (App e x)\<cdot>n = CCexp e\<cdot>(inc\<cdot>n) \<squnion> ccProd (fv e) {x}"
+  "CCexp (App e x)\<cdot>n = CCexp e\<cdot>(inc\<cdot>n) \<squnion> ccProd {x} (insert x (fv e))"
   "CCexp (Let \<Gamma> e)\<cdot>n = cc_restr (fv (Let \<Gamma> e)) (CCfix \<Gamma>\<cdot>(Aexp e\<cdot>n, CCexp e\<cdot>n))"
 unfolding Aexp_def CCexp_def CCfix_def by (simp add: beta_cfun)+
 
